nice!

Dcc/Relations.lean
@@ -1,15 +1,131 @@
 /-
+Application is, in some sense, interpretation of our combinators.
 
+K does not supply new proof information, so application is not required.
+β x.
+
+TODO:
+- correct ValidJudgment proofs using new inference rules
+- fix simp lemmas so as to be cleaner
+- S type
+ -  S induces application, so we will need to decide how that works
+- What is a proof of ∶ T x?
+  - The ValidJudgment constructor
+  - We should be able to refer to these by names, though
+  - This suggests we should be able to improve the judgment rule for app
+
+(∶ interpretation term), term is the proof.
+
+⊢ reduced interpretation₁ interpretation₂
+
+⊢ goal fn x
+
+- our current calculus reduction rules are quite unrestricted.
+we want the typing judgments to be essentially elided after one layer
+so that we can use normal SK.
+
+Note:
+⊢ goal f x should somehow carry its components down
+
+⊢ goal f x can be replaced with just
+
+(∶ (Pi
+
+⊢ gets encoded in the rule for S itself.
+
+S should encode its requirements in its reduction rule.
+
+K should stya the same. It doesn't care.
+
+⊢ (∶ Ttf Tf) (∶ Ttx Tx) (f : Tf) (x : Tx)
+
+Ideas:
+- only encode typing judgments at the highest level of application
+- reduction rules carry these down
+- this happens inside the rule for S
+- also happens in the judgment rule for app
+- we should assume in app rule that Pi has already been substituted.
+- it would be cool to be able to explicit supply proofs of ∶ T x
+  - although these should be inferrable by the type-checker
+
+ValidJudgment f ⸨Pi cod dom⸩
+ValidJudgment x cod
+ValidJudgment ⸨f x⸩ ⸨∶ ⸨dom x⸩ ⸨f x⸩⸩ ⸨f x⸩
+
+S (∶ Pi Tx cod) (∶ (Pi Tx cod)) (∶ Tx x)
+
+Then, S.type becomes
+
+Prop → Prop → Prop → Prop
+
+⊢ becomes unnecessary. we can also encode the dependency in K's reduction rule, I think,
+although this is also unnecessary.
+
+We also ought to improve substitution for Pi
+
+so that we don't need to invoke S in the type for K.
+
+K : Prop → Prop → Prop.
+
+fst / snd have no use now.
+
+fst / snd are just Prop → Prop → Prop, respectively.
+
+snd : (Prop → Prop) → Prop → Prop
+fst : Prop → Prop
+
+Then, Pi becomes substitution as we always thought.
+
+Composition is pretty natural on snd / fst now.
+
+Composition is not necessary, since π is an argument to snd.
+
+K : Pi (: Ty Prop) (Pi (snd fst) K)
+
+This suggests that fst and snd should work on types.
+
+- we should have some clever reduction rule for judgments.
+- we substitute just x in. term, not its type.
+
+this removes need for fst / snd.
+
+Pi substitution rule should not substitute dom.
+
+we should make this on-demand with S.
+
+position of judgments feels like it changes form in to out,
+but this is fine, since it mirrors the substitution rule.
+
+S isn't guaranteed to produce a not-stuck expression
+even if we type-check it.
+
+we need to make sure that f and g line up better.
+
+S as out type still makes sense, but g and x
+should be term arguments, not prop.
+
+This suggests, again, that the sustitution rule should be upgraded.
+
+fst and snd should be operations on judgments
+
+if we can get fst on Pi, that would be nice, too.
+
+It would be really nice for Pi to take Prop arguments.
+we can do that.
+
+fst (∶ α x) = (∶ Ty α)
+
+fst should also work on Pi, probably.
 -/
 
 inductive Expr where
   | Pi    : Expr
   | S     : Expr
   | K     : Expr
+  | I     : Expr
   | judge : Expr
   | type  : Expr
   | prop  : Expr
-  | vdash : Expr
   | fst   : Expr
   | snd   : Expr
   | app   : Expr → Expr → Expr
@@ -22,58 +138,53 @@ notation "Π'" => Expr.Pi
 notation "Ty" => Expr.type
 notation "Prp" => Expr.prop
 notation "∶" => Expr.judge
-notation "⊢" => Expr.vdash
 
 macro_rules
   | `(⸨$f:term $x:term⸩) => `(Expr.app $f $x)
   | `(⸨ $f $x:term $args:term*⸩) => `(⸨ (Expr.app $f $x) $args*⸩)
 
 inductive IsStep : Expr → Expr → Prop
-  | k      : IsStep ⸨K α β x y⸩ x
-  | k'     : IsStep ⸨K x y⸩ x
-  | s      : IsStep ⸨S x y z⸩ ⸨⸨x z⸩ ⸨y z⸩⸩
-  | fst    : IsStep ⸨fst ⸨∶ T x⸩⸩ T
-  | snd    : IsStep ⸨snd ⸨∶ T x⸩⸩ x
+  | k      : IsStep ⸨K x y⸩ x
+  | s      : IsStep ⸨S ⸨∶ ⸨Pi α cod⸩ f⸩ ⸨∶ ⸨Pi α cod⸩ g⸩ ⸨∶ α x⸩⸩
+    ⸨∶
+      ⸨cod ⸨∶ α x⸩ ⸨g ⸨∶ α x⸩⸩⸩
+      ⸨f ⸨∶ α x⸩ ⸨g ⸨∶ α x⸩⸩⸩
+    ⸩
+  | i      : IsStep ⸨I x⸩ x
+  | fst    : IsStep ⸨fst π ⸨∶ α x⸩⸩ ⸨π ⸨∶ Ty α⸩⸩
+  | snd    : IsStep ⸨snd π ⸨∶ α x⸩⸩ ⸨π x⸩
+  | fstπ   : IsStep ⸨fst π ⸨Π' dom cod⸩⸩ ⸨π dom⸩
+  | sndπ   : IsStep ⸨snd π ⸨Π' dom cod⸩⸩ ⸨π cod⸩
+  | pi     : IsStep ⸨⸨Pi dom cod⸩ x⸩ ⸨Pi ⸨dom x⸩ ⸨cod x⸩⸩
   | left   : IsStep f f' → IsStep ⸨f x⸩ ⸨f' x⸩
   | right  : IsStep x x' → IsStep ⸨f x⸩ ⸨f x'⸩
 
 inductive DefEq : Expr → Expr → Prop
   | refl    : DefEq a a
-  | symm    : DefEq e e'
-    → DefEq e' e
+  | symm    : DefEq e e'  → DefEq e' e
   | step    : IsStep e e' → DefEq e e'
   | trans   : DefEq e₁ e₂ → DefEq e₂ e₃ → DefEq e₁ e₃
   | left    : DefEq f f'  → DefEq ⸨f x⸩ ⸨f' x⸩
   | right   : DefEq x x'  → DefEq ⸨f x⸩ ⸨f x'⸩
 
-abbrev B := ⸨S ⸨K S⸩ K⸩
-abbrev C := ⸨S ⸨S ⸨K ⸨S ⸨K S⸩ K⸩⸩ S⸩ ⸨K K⸩⸩
-abbrev I := ⸨S K K⸩
-
-infixr:90 " ∘ " => (fun f g => ⸨B f g⸩)
-
 /-
-Nondependent interpretation of K.
-
-This is fine, since in dependent K:
-K : ∀ (α : Type) (β : α → Type) (x : α) (y : β x), α,
-
-The type of y is not determined by anything. Its type is not under a ∀ binder.
-It should be inferrable given it is an argument of type Prop.
-
-K : (∶ Prop) → (∶ Prop) → (∶ α (K x y))
-⸨∶ α ⸨K ⸨∶ α x⸩ ⸨∶ β y⸩⸩⸩
+K type:
+  K : Prop → Prop → Prop
+  K x y = x
 -/
 def K'.type : Expr :=
-  ⸨Π' ⸨∶ Prp⸩ (⸨Π' ⸨∶ Prp⸩⸩ ∘ (K ∘ fst))⸩
+  ⸨Π' ⸨∶ Ty Prp⸩ ⸨Π' ⸨K ⸨∶ Ty Prp⸩⸩ K⸩⸩
 
 /-
-x : ∀ (x : α) (y : β x), γ x y
-x ≅ Pi α (S nu
-S : (x = (∶ Prop)) → (∶ 
+S type:
+  S : (x : Prop) → (fst x : Prp) → Prop → Prop
+  fst x is a Pi type, Pi dom cod. fst fst x is α in (x : α)
+  S (∶ (Pi α cod) f) (∶ (Pi α cod) g) (∶ α x) = (∶
+    (cod (∶ α x) (g (∶ α x)))
+    (f (∶ α x) (g (∶ α x))))
 -/
 def S.type : Expr :=
-  sorry
+  ⸨Π' ⸨∶ Ty Prp⸩ ⸨Π' ⸨fst I⸩ ⸨Π' ⸨fst ⸨fst K⸩⸩ S⸩⸩⸩
 
 /-
 (: T x) : Prop
@@ -89,7 +200,7 @@ def judge.type : Expr :=
 
 inductive ValidJudgment : Expr → Expr → Prop
   | app   : ValidJudgment ⸨∶ ⸨Π' dom cod⸩ f⸩ f
-    → ValidJudgment ⸨dom x⸩ x
+    → ValidJudgment ⸨∶ dom x⸩ x
     → ValidJudgment ⸨∶ ⸨cod x⸩ ⸨f x⸩⸩ ⸨f x⸩
   | ty    : ValidJudgment ⸨∶ Ty Ty⸩ Ty
   | prp   : ValidJudgment ⸨∶ Ty Prp⸩ Prp
@@ -127,7 +238,12 @@ macro_rules
 
     `(tactic| $[$nms];*)
 
-@[simp] theorem S.step : DefEq ⸨S x y z⸩ s' ↔ DefEq s' ⸨⸨x z⸩ ⸨y z⸩⸩ := by
+@[simp] theorem defeq.refl : DefEq x x := DefEq.refl
+
+@[simp] theorem defeq.trans : DefEq a b → DefEq b c → DefEq a c := DefEq.trans
+
+@[simp] theorem S.step :  DefEq ⸨S x y z⸩ s' = DefEq s' ⸨⸨x z⸩ ⸨y z⸩⸩ := by
+  ext
   constructor
   intro h
   defeq symm, trans, symm, step
@@ -139,20 +255,22 @@ macro_rules
   defeq symm
   assumption
 
-@[simp] theorem K.step : DefEq ⸨K x y⸩ k' ↔ DefEq k' x := by
+@[simp] theorem K.step : DefEq ⸨K x y⸩ k' = DefEq k' x := by
+  ext
   constructor
   intro h
   defeq trans, symm
   exact h
   defeq step
-  step k'
+  step k
   intro h
   defeq trans, step
-  step k'
+  step k
   defeq symm
   exact h
 
-@[simp] theorem B.step : DefEq ⸨B f g x⸩ b' ↔ DefEq b' ⸨f ⸨g x⸩⸩ := by
+@[simp] theorem B.step : DefEq ⸨B f g x⸩ b' = DefEq b' ⸨f ⸨g x⸩⸩ := by
+  ext
   constructor
   intro h
   defeq trans, symm
@@ -162,22 +280,21 @@ macro_rules
   step left, left
   step s
   defeq trans, step
-  step left, left, left, k'
+  step left, left, left, k
   simp
   defeq symm, left
   simp
-  defeq refl
   intro h
   defeq symm, trans
   exact h
   defeq symm, trans, step
   step left, left, s
   defeq trans, left, left, left, step
-  step k'
+  step k
   defeq trans, step
   step s
   defeq left, step
-  step k'
+  step k
 
 @[simp] theorem C.step : DefEq ⸨C x y z⸩ c' ↔ DefEq c' ⸨x z y⸩ := by
   constructor
@@ -194,9 +311,7 @@ macro_rules
   simp
   defeq symm, trans, left
   simp
-  defeq refl
-  defeq refl
-  defeq refl
+  defeq refl, refl, refl
   defeq trans, left
   simp
   defeq symm, trans, left
@@ -207,7 +322,6 @@ macro_rules
   simp
   defeq refl
   simp
-  defeq refl
   intro h
   defeq symm, trans
   exact h
@@ -221,9 +335,7 @@ macro_rules
   simp
   defeq symm, trans, left
   simp
-  defeq refl
-  defeq refl
-  defeq refl
+  defeq refl, refl, refl
   defeq trans, left
   simp
   defeq symm, trans, left
@@ -235,12 +347,7 @@ macro_rules
   simp
   defeq symm, trans, right
   simp
-  defeq refl
-  defeq refl
-
-theorem defeq.refl : DefEq x x := DefEq.refl
-
-theorem defeq.symm : DefEq x y ↔ DefEq y x := ⟨DefEq.symm, DefEq.symm⟩
+  defeq refl, refl
 
 theorem K.preservation : ValidJudgment ⸨∶ Ty α⸩ α
   → ValidJudgment ⸨∶ Ty β⸩ β
